proof/extraction/XMSS_IMPL_PP.ec
@@ -28,13 +28,13 @@ module Mp(SC:Syscall_t) = {
     return (out);
   }
 
-  proc __ull_to_bytes_4 (out:W8.t Array4.t, in_0:W64.t) : W8.t Array4.t = {
+  proc __ull_to_bytes_2 (out:W8.t Array2.t, in_0:W64.t) : W8.t Array2.t = {
     var aux: int;
 
     var i:int;
 
     aux <- (- 1);
-    i <- (4 - 1);
+    i <- (2 - 1);
     while (aux < i) {
       out.[i] <- (truncateu8 in_0);
       in_0 <- (in_0 `>>` (W8.of_int 8));
@@ -58,13 +58,13 @@ module Mp(SC:Syscall_t) = {
     return (out);
   }
 
-  proc __ull_to_bytes_2 (out:W8.t Array2.t, in_0:W64.t) : W8.t Array2.t = {
+  proc __ull_to_bytes_4 (out:W8.t Array4.t, in_0:W64.t) : W8.t Array4.t = {
     var aux: int;
 
     var i:int;
 
     aux <- (- 1);
-    i <- (2 - 1);
+    i <- (4 - 1);
     while (aux < i) {
       out.[i] <- (truncateu8 in_0);
       in_0 <- (in_0 `>>` (W8.of_int 8));
@@ -287,22 +287,6 @@ module Mp(SC:Syscall_t) = {
     return ();
   }
 
-  proc __memcpy_u8pu8_32 (out:W64.t, offset:W64.t, in_0:W8.t Array32.t) : 
-  W64.t * W64.t = {
-
-    var i:W64.t;
-
-    i <- (W64.of_int 0);
-
-    while ((i \ult (W64.of_int 32))) {
-      Glob.mem <-
-      storeW8 Glob.mem (W64.to_uint (out + offset)) (in_0.[(W64.to_uint i)]);
-      offset <- (offset + (W64.of_int 1));
-      i <- (i + (W64.of_int 1));
-    }
-    return (out, offset);
-  }
-
   proc __memcpy_u8pu8_4 (out:W64.t, offset:W64.t, in_0:W8.t Array4.t) : 
   W64.t * W64.t = {
 
@@ -319,10 +303,19 @@ module Mp(SC:Syscall_t) = {
     return (out, offset);
   }
 
-  proc _memcpy_u8pu8_32 (out:W64.t, offset:W64.t, in_0:W8.t Array32.t) : 
+  proc __memcpy_u8pu8_32 (out:W64.t, offset:W64.t, in_0:W8.t Array32.t) : 
   W64.t * W64.t = {
 
-    (out, offset) <@ __memcpy_u8pu8_32 (out, offset, in_0);
+    var i:W64.t;
+
+    i <- (W64.of_int 0);
+
+    while ((i \ult (W64.of_int 32))) {
+      Glob.mem <-
+      storeW8 Glob.mem (W64.to_uint (out + offset)) (in_0.[(W64.to_uint i)]);
+      offset <- (offset + (W64.of_int 1));
+      i <- (i + (W64.of_int 1));
+    }
     return (out, offset);
   }
 
@@ -333,15 +326,10 @@ module Mp(SC:Syscall_t) = {
     return (out, offset);
   }
 
-  proc _x_memcpy_u8pu8_32 (out:W64.t, offset:W64.t, in_0:W8.t Array32.t) : 
+  proc _memcpy_u8pu8_32 (out:W64.t, offset:W64.t, in_0:W8.t Array32.t) : 
   W64.t * W64.t = {
 
-    out <- out;
-    offset <- offset;
-    in_0 <- in_0;
-    (out, offset) <@ _memcpy_u8pu8_32 (out, offset, in_0);
-    out <- out;
-    offset <- offset;
+    (out, offset) <@ __memcpy_u8pu8_32 (out, offset, in_0);
     return (out, offset);
   }
 
@@ -352,6 +340,18 @@ module Mp(SC:Syscall_t) = {
     offset <- offset;
     in_0 <- in_0;
     (out, offset) <@ _memcpy_u8pu8_4 (out, offset, in_0);
+    out <- out;
+    offset <- offset;
+    return (out, offset);
+  }
+
+  proc _x_memcpy_u8pu8_32 (out:W64.t, offset:W64.t, in_0:W8.t Array32.t) : 
+  W64.t * W64.t = {
+
+    out <- out;
+    offset <- offset;
+    in_0 <- in_0;
+    (out, offset) <@ _memcpy_u8pu8_32 (out, offset, in_0);
     out <- out;
     offset <- offset;
     return (out, offset);
@@ -817,6 +817,7 @@ module Mp(SC:Syscall_t) = {
   W8.t Array32.t * W32.t Array8.t = {
 
     out <- out;
+    steps <- steps;
     pub_seed <- pub_seed;
     addr <- addr;
     (out, addr) <@ _gen_chain_inplace (out, steps, pub_seed, addr);
@@ -825,13 +826,25 @@ module Mp(SC:Syscall_t) = {
     return (out, addr);
   }
 
-  proc __csum (msg_base_w:W32.t Array67.t) : W64.t = {
+  proc __wots_checksum (csum_base_w:W32.t Array3.t,
+                        msg_base_w:W32.t Array67.t) : W32.t Array3.t = {
+
+    var t_list : W32.t list;
 
     var csum:W64.t;
     var i:W64.t;
     var t:W64.t;
     var u:W64.t;
-
+    var k:int;
+    var _of_:bool;
+    var _cf_:bool;
+    var _sf_:bool;
+    var _zf_:bool;
+    var csum_bytes:W8.t Array2.t;
+    var csum_bytes_p:W8.t Array2.t;
+    var  _0:bool;
+    csum_bytes <- witness;
+    csum_bytes_p <- witness;
     csum <- (W64.of_int 0);
     i <- (W64.of_int 0);
 
@@ -842,27 +855,6 @@ module Mp(SC:Syscall_t) = {
       csum <- (csum + t);
       i <- (i + (W64.of_int 1));
     }
-    return (csum);
-  }
-
-  proc __wots_checksum (csum_base_w:W32.t Array3.t,
-                        msg_base_w:W32.t Array67.t) : W32.t Array3.t = {
-
-    var t_list : W32.t list;
-
-    var csum:W64.t;
-    var k:int;
-    var u:W64.t;
-    var _of_:bool;
-    var _cf_:bool;
-    var _sf_:bool;
-    var _zf_:bool;
-    var csum_bytes:W8.t Array2.t;
-    var csum_bytes_p:W8.t Array2.t;
-    var  _0:bool;
-    csum_bytes <- witness;
-    csum_bytes_p <- witness;
-    csum <@ __csum (msg_base_w);
     k <- ((3 * 4) %% 8);
     u <- (W64.of_int 8);
     u <- (u - (W64.of_int k));
@@ -1005,6 +997,7 @@ module Mp(SC:Syscall_t) = {
 
     var lengths:W32.t Array67.t;
     var i:int;
+    var chain:W32.t;
     var start:W32.t;
     var steps:W32.t;
     var t:W64.t;
@@ -1013,7 +1006,8 @@ module Mp(SC:Syscall_t) = {
     lengths <@ __chain_lengths_ (lengths, msg);
     i <- 0;
     while (i < 67) {
-      addr <@ __set_chain_addr (addr, (W32.of_int i));
+      chain <- (W32.of_int i);
+      addr <@ __set_chain_addr (addr, chain);
 
       start <- lengths.[i];
       steps <- (W32.of_int (16 - 1));
