proof/correctness/Correctness_Mem.ec
@@ -9,6 +9,10 @@ require import XMSS_IMPL XMSS_IMPL_PP.
 
 require import Utils. (* valid_ptr predicate *)
 
+(******************************************************************************)
+(******************               MEMSET                          *************)
+(******************************************************************************)
+
 lemma memset_4_post (input : W8.t Array4.t, v : W8.t) :
     hoare [M(Syscall).__memset_u8_4 : arg=(input, v) ==> 
      (forall (k : int), 0 <= k < 4 => (res.[k] = v))].
@@ -77,24 +81,49 @@ while (
     + move => mem ????? k *. rewrite /loadW8. admit.
 qed.
 
+(******************************************************************************)
+(******************               MEMCPY                          *************)
+(******************************************************************************)
+lemma memcpy_ptr_correct (ptr : W64.t):
+    hoare [Mp(Syscall)._x_memcpy_u8u8p : 
+      arg.`2 = ptr /\  
+      0 <= (to_uint ptr) + 32 <= W64.modulus /\
+      0 <= to_uint ptr ==>
+        res = Array32.init (fun (i : int) => loadW8 Glob.mem (to_uint ptr + i))].
+proof.
+proc.
+inline *.
+wp ; sp.
+while (
+  0 <= i <= 32 /\
+  0 <= to_uint in_ptr{hr} + 32 <= W64.modulus /\
+  forall (k : int), 0 <= k < i => (out1.[k] = loadW8 Glob.mem ((to_uint ptr) + k))
+) ; auto => />; last first.
+- move => &hr *. split ; first by smt(@JMemory). move => *. apply tP ; smt(@JMemory @Array32).
+- move => &hr *. split ; first by smt(). move => k *. rewrite get_setE 1:/#. case (k = i{hr}); last by smt(@JMemory).
+  move => E0 ; congr. rewrite E0 to_uintD of_uintK //=. admit. (* overflow *)
+qed.
 
-lemma memcpy_ptr_post (ptr : W64.t, o : W8.t Array32.t):
-    hoare [M(Syscall).__memcpy_u8u8p : 
-      arg=(o, ptr) /\ valid_ptr ptr (W64.of_int 32) ==>
-            forall (k : int), 0 <= k < 32 => res.[k] = loadW8 Glob.mem (to_uint ptr + k)].
+
+lemma  memcpy_post (x : W8.t Array32.t) :
+    hoare [M(Syscall).__memcpy_u8u8_32_32 : arg.`2 = x ==> res = x].
 proof.
 proc.
 while (
-  #pre /\
-  0 <= i <= 32 /\
-  (forall (k : int), 0 <= k < i => out.[k] = loadW8 Glob.mem ((to_uint in_ptr) + k))
-) ; auto => />.
-- move => &hr * ; do split.
-    + rewrite /loadW8. admit.
-    + smt().
-    + smt().
-    + move => k *. rewrite /loadW8 get_setE. smt(). case ( k = i{hr}).
-      * move => H0. congr. rewrite to_uintD_small ; [ admit | rewrite of_uintK ; congr ; smt() ].
-      * move => ? ; smt(@JMemory).
-- move => &hr * ; do split ; by smt().
+  0 <= to_uint i <= 32 /\
+  (forall (k : int), 0 <= k < to_uint i => (out.[k] = in_0.[k]))
+); last first.
+- auto => /> *. split ; first by smt(). progress. rewrite tP. move => *. smt.
+- auto => /> &hr *. do split; 1,2: by smt(@W64). move => k *. rewrite get_setE. smt(@W64). case (k = to_uint i{hr}).
+    + move => E0 ; by rewrite E0.
+    + move => E0. smt.
+qed.
+
+lemma _x_memcpy_u8u8_post (x : W8.t Array32.t) :
+    hoare [M(Syscall)._x_memcpy_u8u8_32_32 : arg.`2 = x ==> res = x].
+proof.
+proc ; inline M(Syscall)._memcpy_u8u8_32_32.
+wp ; sp.
+ecall (memcpy_post in_00).
+skip => /> *.
 qed.
