proof/correctness/Repr.ec
@@ -1,0 +1,66 @@
+pragma Goals : printall.
+
+require import AllCore List.
+from Jasmin require import JModel.
+
+require import Address Wots XMSS_MT_PRF.
+require import XMSS_IMPL XMSS_IMPL_PP.
+
+require import Array32 Array2144.
+
+(* 
+    Operators to convert impl representation (i.e. arrays) to spec representation and
+    predicates for equality 
+
+    Enc :: Spec -> Impl
+    Dec :: Impl -> Spec
+    
+    Dec . Enc = Id
+*)
+
+(**************************************************************************************************)
+(*******************                        MEM                                 *******************)
+(**************************************************************************************************)
+
+(* W8 list w/32 elements loaded from memory *)
+op load_mem_w8_list32 (mem : global_mem_t) (ptr : W64.t) : W8.t list =
+    mkseq (fun (i : int) => loadW8 mem (to_uint ptr + i)) 32.
+
+op load_mem_w8_array32 (mem : global_mem_t) (ptr : W64.t) : W8.t Array32.t =
+    Array32.init (fun (i : int) => loadW8 mem (to_uint ptr + i)).
+
+lemma load_mem_list_array_32 (mem : global_mem_t) (ptr : W64.t) :
+    load_mem_w8_list32 mem ptr = to_list (load_mem_w8_array32 mem ptr).
+proof.
+rewrite /load_mem_w8_list32 /load_mem_w8_array32.
+apply (eq_from_nth witness) ; [ rewrite /to_list !size_mkseq //= | smt(@List @Array32) ].
+qed.
+
+
+(**************************************************************************************************)
+(*******************                        HASH                                *******************)
+(**************************************************************************************************)
+
+
+(**************************************************************************************************)
+(*******************                        WOTS                                *******************)
+(**************************************************************************************************)
+
+op enc_wots_sk (sk : wots_sk) : W8.t Array2144.t =
+    Array2144.of_list witness (flatten sk).
+
+
+pred eq_wots_sk (sk_impl : W8.t Array2144.t) (sk_spec : wots_sk) = 
+    flatten sk_spec = (to_list sk_impl).
+
+op enc_wots_pk (pk : wots_pk) : W8.t Array2144.t =
+    Array2144.of_list witness (flatten pk).
+
+
+pred eq_wots_pk (pk_impl : W8.t Array2144.t) (pk_spec : wots_pk) = 
+    flatten pk_spec = (to_list pk_impl).
+
+(**************************************************************************************************)
+(*******************                        XNSS                                *******************)
+(**************************************************************************************************)
+
