proof/extraction/XMSS_IMPL.ec
@@ -877,19 +877,19 @@ module M(SC:Syscall_t) = {
     return (out);
   }
   
-  proc __core_hash_96 (out:W8.t Array32.t, in_0:W8.t Array96.t) : W8.t Array32.t = {
-    
-    
-    
-    out <@ __sha256_96 (out, in_0);
-    return (out);
-  }
-  
   proc __core_hash_128 (out:W8.t Array32.t, in_0:W8.t Array128.t) : W8.t Array32.t = {
     
     
     
     out <@ __sha256_128 (out, in_0);
+    return (out);
+  }
+  
+  proc __core_hash_96 (out:W8.t Array32.t, in_0:W8.t Array96.t) : W8.t Array32.t = {
+    
+    
+    
+    out <@ __sha256_96 (out, in_0);
     return (out);
   }
   
@@ -916,6 +916,18 @@ module M(SC:Syscall_t) = {
     in_0 <- in_0;
     out <- out;
     out <@ _core_hash_96 (out, in_0);
+    out <- out;
+    return (out);
+  }
+  
+  proc __core_hash__128 (out:W8.t Array32.t, in_0:W8.t Array128.t) : 
+  W8.t Array32.t = {
+    
+    
+    
+    in_0 <- in_0;
+    out <- out;
+    out <@ _core_hash_128 (out, in_0);
     out <- out;
     return (out);
   }
@@ -961,13 +973,13 @@ module M(SC:Syscall_t) = {
     return (out);
   }
   
-  proc __ull_to_bytes_4 (out:W8.t Array4.t, in_0:W64.t) : W8.t Array4.t = {
+  proc __ull_to_bytes_2 (out:W8.t Array2.t, in_0:W64.t) : W8.t Array2.t = {
     var aux: int;
     
     var i:int;
     
     aux <- (- 1);
-    i <- (4 - 1);
+    i <- (2 - 1);
     while (aux < i) {
       out.[i] <- (truncateu8 in_0);
       in_0 <- (in_0 `>>` (W8.of_int 8));
@@ -991,13 +1003,13 @@ module M(SC:Syscall_t) = {
     return (out);
   }
   
-  proc __ull_to_bytes_2 (out:W8.t Array2.t, in_0:W64.t) : W8.t Array2.t = {
+  proc __ull_to_bytes_4 (out:W8.t Array4.t, in_0:W64.t) : W8.t Array4.t = {
     var aux: int;
     
     var i:int;
     
     aux <- (- 1);
-    i <- (2 - 1);
+    i <- (4 - 1);
     while (aux < i) {
       out.[i] <- (truncateu8 in_0);
       in_0 <- (in_0 `>>` (W8.of_int 8));
@@ -1170,20 +1182,6 @@ module M(SC:Syscall_t) = {
     return (out);
   }
   
-  proc __memcpy_u8u8_32_32 (out:W8.t Array32.t, in_0:W8.t Array32.t) : 
-  W8.t Array32.t = {
-    
-    var i:W64.t;
-    
-    i <- (W64.of_int 0);
-    
-    while ((i \ult (W64.of_int 32))) {
-      out.[(W64.to_uint i)] <- in_0.[(W64.to_uint i)];
-      i <- (i + (W64.of_int 1));
-    }
-    return (out);
-  }
-  
   proc __memcpy_u8u8_64_64 (out:W8.t Array64.t, in_0:W8.t Array64.t) : 
   W8.t Array64.t = {
     
@@ -1192,6 +1190,20 @@ module M(SC:Syscall_t) = {
     i <- (W64.of_int 0);
     
     while ((i \ult (W64.of_int 64))) {
+      out.[(W64.to_uint i)] <- in_0.[(W64.to_uint i)];
+      i <- (i + (W64.of_int 1));
+    }
+    return (out);
+  }
+  
+  proc __memcpy_u8u8_32_32 (out:W8.t Array32.t, in_0:W8.t Array32.t) : 
+  W8.t Array32.t = {
+    
+    var i:W64.t;
+    
+    i <- (W64.of_int 0);
+    
+    while ((i \ult (W64.of_int 32))) {
       out.[(W64.to_uint i)] <- in_0.[(W64.to_uint i)];
       i <- (i + (W64.of_int 1));
     }
@@ -1207,21 +1219,21 @@ module M(SC:Syscall_t) = {
     return (out);
   }
   
-  proc _memcpy_u8u8_32_32 (out:W8.t Array32.t, in_0:W8.t Array32.t) : 
-  W8.t Array32.t = {
-    
-    
-    
-    out <@ __memcpy_u8u8_32_32 (out, in_0);
-    return (out);
-  }
-  
   proc _memcpy_u8u8_64_64 (out:W8.t Array64.t, in_0:W8.t Array64.t) : 
   W8.t Array64.t = {
     
     
     
     out <@ __memcpy_u8u8_64_64 (out, in_0);
+    return (out);
+  }
+  
+  proc _memcpy_u8u8_32_32 (out:W8.t Array32.t, in_0:W8.t Array32.t) : 
+  W8.t Array32.t = {
+    
+    
+    
+    out <@ __memcpy_u8u8_32_32 (out, in_0);
     return (out);
   }
   
@@ -1237,18 +1249,6 @@ module M(SC:Syscall_t) = {
     return (out);
   }
   
-  proc _x_memcpy_u8u8_32_32 (out:W8.t Array32.t, in_0:W8.t Array32.t) : 
-  W8.t Array32.t = {
-    
-    
-    
-    out <- out;
-    in_0 <- in_0;
-    out <@ _memcpy_u8u8_32_32 (out, in_0);
-    out <- out;
-    return (out);
-  }
-  
   proc _x_memcpy_u8u8_64_64 (out:W8.t Array64.t, in_0:W8.t Array64.t) : 
   W8.t Array64.t = {
     
@@ -1257,6 +1257,18 @@ module M(SC:Syscall_t) = {
     out <- out;
     in_0 <- in_0;
     out <@ _memcpy_u8u8_64_64 (out, in_0);
+    out <- out;
+    return (out);
+  }
+  
+  proc _x_memcpy_u8u8_32_32 (out:W8.t Array32.t, in_0:W8.t Array32.t) : 
+  W8.t Array32.t = {
+    
+    
+    
+    out <- out;
+    in_0 <- in_0;
+    out <@ _memcpy_u8u8_32_32 (out, in_0);
     out <- out;
     return (out);
   }
@@ -1365,22 +1377,6 @@ module M(SC:Syscall_t) = {
     return ();
   }
   
-  proc __memcpy_u8pu8_32 (out:W64.t, offset:W64.t, in_0:W8.t Array32.t) : 
-  W64.t * W64.t = {
-    
-    var i:W64.t;
-    
-    i <- (W64.of_int 0);
-    
-    while ((i \ult (W64.of_int 32))) {
-      Glob.mem <-
-      storeW8 Glob.mem (W64.to_uint (out + offset)) (in_0.[(W64.to_uint i)]);
-      offset <- (offset + (W64.of_int 1));
-      i <- (i + (W64.of_int 1));
-    }
-    return (out, offset);
-  }
-  
   proc __memcpy_u8pu8_4 (out:W64.t, offset:W64.t, in_0:W8.t Array4.t) : 
   W64.t * W64.t = {
     
@@ -1397,12 +1393,19 @@ module M(SC:Syscall_t) = {
     return (out, offset);
   }
   
-  proc _memcpy_u8pu8_32 (out:W64.t, offset:W64.t, in_0:W8.t Array32.t) : 
+  proc __memcpy_u8pu8_32 (out:W64.t, offset:W64.t, in_0:W8.t Array32.t) : 
   W64.t * W64.t = {
     
+    var i:W64.t;
     
+    i <- (W64.of_int 0);
     
-    (out, offset) <@ __memcpy_u8pu8_32 (out, offset, in_0);
+    while ((i \ult (W64.of_int 32))) {
+      Glob.mem <-
+      storeW8 Glob.mem (W64.to_uint (out + offset)) (in_0.[(W64.to_uint i)]);
+      offset <- (offset + (W64.of_int 1));
+      i <- (i + (W64.of_int 1));
+    }
     return (out, offset);
   }
   
@@ -1415,17 +1418,12 @@ module M(SC:Syscall_t) = {
     return (out, offset);
   }
   
-  proc _x_memcpy_u8pu8_32 (out:W64.t, offset:W64.t, in_0:W8.t Array32.t) : 
+  proc _memcpy_u8pu8_32 (out:W64.t, offset:W64.t, in_0:W8.t Array32.t) : 
   W64.t * W64.t = {
     
     
     
-    out <- out;
-    offset <- offset;
-    in_0 <- in_0;
-    (out, offset) <@ _memcpy_u8pu8_32 (out, offset, in_0);
-    out <- out;
-    offset <- offset;
+    (out, offset) <@ __memcpy_u8pu8_32 (out, offset, in_0);
     return (out, offset);
   }
   
@@ -1438,6 +1436,20 @@ module M(SC:Syscall_t) = {
     offset <- offset;
     in_0 <- in_0;
     (out, offset) <@ _memcpy_u8pu8_4 (out, offset, in_0);
+    out <- out;
+    offset <- offset;
+    return (out, offset);
+  }
+  
+  proc _x_memcpy_u8pu8_32 (out:W64.t, offset:W64.t, in_0:W8.t Array32.t) : 
+  W64.t * W64.t = {
+    
+    
+    
+    out <- out;
+    offset <- offset;
+    in_0 <- in_0;
+    (out, offset) <@ _memcpy_u8pu8_32 (out, offset, in_0);
     out <- out;
     offset <- offset;
     return (out, offset);
@@ -1656,7 +1668,7 @@ module M(SC:Syscall_t) = {
     buf <- Array128.init
            (fun i => if (32 + 32) <= i < (32 + 32) + 64
            then aux_0.[i-(32 + 32)] else buf.[i]);
-    out <@ __core_hash_128 (out, buf);
+    out <@ __core_hash__128 (out, buf);
     return (out);
   }
   
@@ -2051,6 +2063,7 @@ module M(SC:Syscall_t) = {
     
     
     out <- out;
+    steps <- steps;
     pub_seed <- pub_seed;
     addr <- addr;
     (out, addr) <@ _gen_chain_inplace (out, steps, pub_seed, addr);
@@ -2063,9 +2076,11 @@ module M(SC:Syscall_t) = {
   W32.t Array67.t = {
     
     var in_0:W64.t;
+    var out:W64.t;
     var bits:W64.t;
-    var total:W32.t;
-    var i:W64.t;
+    var consumed:W64.t;
+    var total:W8.t;
+    var total_32:W32.t;
     var _of_:bool;
     var _cf_:bool;
     var _sf_:bool;
@@ -2073,23 +2088,26 @@ module M(SC:Syscall_t) = {
     var  _0:bool;
     
     in_0 <- (W64.of_int 0);
+    out <- (W64.of_int 0);
     bits <- (W64.of_int 0);
-    total <- (W32.of_int 0);
-    i <- (W64.of_int 0);
+    consumed <- (W64.of_int 0);
     
-    while ((i \ult (W64.of_int 67))) {
+    while ((consumed \ult (W64.of_int 67))) {
       if ((bits = (W64.of_int 0))) {
-        total <- (zeroextu32 input.[(W64.to_uint in_0)]);
+        total <- input.[(W64.to_uint in_0)];
         in_0 <- (in_0 + (W64.of_int 1));
         bits <- (bits + (W64.of_int 8));
       } else {
         
       }
       bits <- (bits - (W64.of_int 4));
-      (_of_, _cf_, _sf_,  _0, _zf_, total) <- SHR_32 total (truncateu8 bits);
-      total <- (total `&` (W32.of_int (16 - 1)));
-      output.[(W64.to_uint i)] <- total;
-      i <- (i + (W64.of_int 1));
+      total_32 <- (zeroextu32 total);
+      (_of_, _cf_, _sf_,  _0, _zf_, total_32) <- SHR_32 total_32
+      (truncateu8 bits);
+      total_32 <- (total_32 `&` (W32.of_int (16 - 1)));
+      output.[(W64.to_uint out)] <- total_32;
+      out <- (out + (W64.of_int 1));
+      consumed <- (consumed + (W64.of_int 1));
     }
     return (output);
   }
@@ -2097,9 +2115,11 @@ module M(SC:Syscall_t) = {
   proc __base_w_3_2 (output:W32.t Array3.t, input:W8.t Array2.t) : W32.t Array3.t = {
     
     var in_0:W64.t;
+    var out:W64.t;
     var bits:W64.t;
-    var total:W32.t;
-    var i:W64.t;
+    var consumed:W64.t;
+    var total:W8.t;
+    var total_32:W32.t;
     var _of_:bool;
     var _cf_:bool;
     var _sf_:bool;
@@ -2107,34 +2127,47 @@ module M(SC:Syscall_t) = {
     var  _0:bool;
     
     in_0 <- (W64.of_int 0);
+    out <- (W64.of_int 0);
     bits <- (W64.of_int 0);
-    total <- (W32.of_int 0);
-    i <- (W64.of_int 0);
+    consumed <- (W64.of_int 0);
     
-    while ((i \ult (W64.of_int 3))) {
+    while ((consumed \ult (W64.of_int 3))) {
       if ((bits = (W64.of_int 0))) {
-        total <- (zeroextu32 input.[(W64.to_uint in_0)]);
+        total <- input.[(W64.to_uint in_0)];
         in_0 <- (in_0 + (W64.of_int 1));
         bits <- (bits + (W64.of_int 8));
       } else {
         
       }
       bits <- (bits - (W64.of_int 4));
-      (_of_, _cf_, _sf_,  _0, _zf_, total) <- SHR_32 total (truncateu8 bits);
-      total <- (total `&` (W32.of_int (16 - 1)));
-      output.[(W64.to_uint i)] <- total;
-      i <- (i + (W64.of_int 1));
+      total_32 <- (zeroextu32 total);
+      (_of_, _cf_, _sf_,  _0, _zf_, total_32) <- SHR_32 total_32
+      (truncateu8 bits);
+      total_32 <- (total_32 `&` (W32.of_int (16 - 1)));
+      output.[(W64.to_uint out)] <- total_32;
+      out <- (out + (W64.of_int 1));
+      consumed <- (consumed + (W64.of_int 1));
     }
     return (output);
   }
   
-  proc __csum (msg_base_w:W32.t Array67.t) : W64.t = {
+  proc __wots_checksum (csum_base_w:W32.t Array3.t,
+                        msg_base_w:W32.t Array67.t) : W32.t Array3.t = {
     
     var csum:W64.t;
     var i:W64.t;
     var t:W64.t;
     var u:W64.t;
-    
+    var k:int;
+    var _of_:bool;
+    var _cf_:bool;
+    var _sf_:bool;
+    var _zf_:bool;
+    var csum_bytes:W8.t Array2.t;
+    var csum_bytes_p:W8.t Array2.t;
+    var  _0:bool;
+    csum_bytes <- witness;
+    csum_bytes_p <- witness;
     csum <- (W64.of_int 0);
     i <- (W64.of_int 0);
     
@@ -2145,25 +2178,6 @@ module M(SC:Syscall_t) = {
       csum <- (csum + t);
       i <- (i + (W64.of_int 1));
     }
-    return (csum);
-  }
-  
-  proc __wots_checksum (csum_base_w:W32.t Array3.t,
-                        msg_base_w:W32.t Array67.t) : W32.t Array3.t = {
-    
-    var csum:W64.t;
-    var k:int;
-    var u:W64.t;
-    var _of_:bool;
-    var _cf_:bool;
-    var _sf_:bool;
-    var _zf_:bool;
-    var csum_bytes:W8.t Array2.t;
-    var csum_bytes_p:W8.t Array2.t;
-    var  _0:bool;
-    csum_bytes <- witness;
-    csum_bytes_p <- witness;
-    csum <@ __csum (msg_base_w);
     k <- ((3 * 4) %% 8);
     u <- (W64.of_int 8);
     u <- (u - (W64.of_int k));
@@ -2308,6 +2322,7 @@ module M(SC:Syscall_t) = {
     
     var lengths:W32.t Array67.t;
     var i:int;
+    var chain:W32.t;
     var start:W32.t;
     var steps:W32.t;
     var t:W64.t;
@@ -2316,7 +2331,8 @@ module M(SC:Syscall_t) = {
     lengths <@ __chain_lengths_ (lengths, msg);
     i <- 0;
     while (i < 67) {
-      addr <@ __set_chain_addr (addr, (W32.of_int i));
+      chain <- (W32.of_int i);
+      addr <@ __set_chain_addr (addr, chain);
       (* Erased call to unspill *)
       start <- lengths.[i];
       steps <- (W32.of_int (16 - 1));
